proof/invariant-abstract/ARM/ArchDetSchedSchedule_AI.thy
@@ -162,8 +162,8 @@ lemma switch_to_idle_thread_ct_not_queued [wp, DetSchedSchedule_AI_assms]:
                          pred_tcb_at_def obj_at_def not_queued_def)
   done
 
-crunch valid_blocked_2[wp]: set_vm_root "\<lambda>s.
-           valid_blocked_2 (ready_queues s) (release_queue s) (kheap s)
+crunch valid_blocked_except_set[wp]: set_vm_root "\<lambda>s.
+           valid_blocked_except_set_2 {} (ready_queues s) (release_queue s) (kheap s)
             (scheduler_action s) thread"
   (wp: crunch_wps simp: crunch_simps)
 
